Pass progress!

Pass.lean
@@ -1,3 +1,4 @@
+import Mathlib.Lean.Expr.Basic
 import Mathlib.Data.ZMod.Defs
 import Mathlib.Data.ZMod.Basic
 
@@ -23,7 +24,7 @@ instance : Sub (Expr p ι) where
 instance : OfNat (Expr p ι) n where
   ofNat := Expr.const n
 
-def Constraints (p ι : Nat) :=
+abbrev Constraints (p ι : Nat) :=
   List (Expr p ι)
 
 /-!
@@ -95,9 +96,24 @@ inductive Constraint.IsRefinedBy : Constraints p ι → Constraints p κ → Pro
           -- ------------------------ ^^^^^^^^^^^^^^^^^^^
           -- This expresses that `env'` is an extension of `env`
           --
+
+          -- TODO: this should also say that `env'` is the *unique* extension
+          --       that satisfies `c₂`
       : IsRefinedBy c₁ c₂
 
 infixl:67 " ⊑ " => Constraint.IsRefinedBy
+
+/-!
+## Simp Automation
+-/
+section Simproc
+
+theorem exists_env_iff {P : Environment _ _ → Prop} :
+    (∃ (env : Environment p (ι + 1)), P env)
+    ↔ (∃ (x : ZMod p) (env : Environment p ι), P (env.append [x].get)) := by
+  sorry
+
+end Simproc
 
 /-!
 ## Example
@@ -126,10 +142,14 @@ example : HigherOrder ⊑ LowerOrder := by
   · intro env
     simp [Constraints.eval, Expr.eval, Environment.restrict]
     grind
+
   · intro env
     simp [Constraints.eval, Expr.eval]
     intro h
 
+    -- The below simplifies the existential quantifier to talk about values `y`
+    -- and `z` rather than abstract environments. For now, we manually copied
+    -- the rest of the statement, but this should be automatically generatable.
     suffices ∃ (y z : ZMod p),
       env 0 * env 0 - y = 0 ∧ y * y - z = 0 ∧ env 0 * z + 1 = 0
     by
@@ -144,7 +164,9 @@ example : HigherOrder ⊑ LowerOrder := by
         --    (in particular, only index `0`), `fin_cases` does a case analasis on
         --    all value for `i`.
         rfl
-      · have : env.append [y, z].get 0 = env 0 := rfl
+      · -- The following rewrites should just follow from simp-lemmas, but
+        -- the API seems to be missing at the moment.
+        have : env.append [y, z].get 0 = env 0 := rfl
         have : env.append [y, z].get 1 = y := rfl
         have : env.append [y, z].get 2 = z := rfl
         simp [*]
@@ -154,11 +176,292 @@ example : HigherOrder ⊑ LowerOrder := by
     simp only [this]
     grind
 
+end Examples
+
+/-!
+## Degree Lowering Pass
+-/
+
+/-!
+### Compute Max Degree
+-/
+
+/-- The maximum degree of a polynomial expression. -/
+def Expr.maxDegree : Expr p ι → Nat
+  | .const _ => 0
+  | .var _ => 1
+  | .sub e₁ e₂ | .add e₁ e₂ => max e₁.maxDegree e₂.maxDegree
+  | .mul e₁ e₂ => e₁.maxDegree + e₂.maxDegree
+
+/-- The maximum degree of a collection of polynomial expressions. -/
+def Constraints.maxDegree (c : Constraints p ι) : Nat :=
+  c.map Expr.maxDegree |>.max? |>.getD 0
+
+/-!
+### Extra Expr API
+-/
+namespace Expr
+
+/--
+Loosen the bounds on the number of free variables in the expression.
+-/
+def castLE (h : ι ≤ κ := by grind) : Expr p ι → Expr p κ
+  | .var i      => .var <| i.castLE h
+  | .const x    => .const x
+  | .add e₁ e₂  => .add e₁.castLE e₂.castLE
+  | .sub e₁ e₂  => .sub e₁.castLE e₂.castLE
+  | .mul e₁ e₂  => .mul e₁.castLE e₂.castLE
+
+@[simp] theorem sizeOf_castLE (e : Expr p ι) (h : ι ≤ κ) :
+    sizeOf (e.castLE h) = sizeOf e := by
+  induction e <;> simp [castLE, *]
+
+@[simp] theorem maxDegree_castLE (e : Expr p ι) (h : ι ≤ κ) :
+    maxDegree (e.castLE h) = e.maxDegree := by
+  induction e <;> simp [castLE, maxDegree, *]
+
+end Expr
+
+/-!
+### Extra Constraints API
+-/
+namespace Constraints
+
+/-- Add a new constraints to a set of constraints -/
+def add : Constraints p ι → Expr p ι → Constraints p ι :=
+  fun c e => c ++ [e]
+
+/-- Loosen the bounds on the free variables of all constraints in a set -/
+def castLE (h : ι ≤ κ := by grind) : Constraints p ι → Constraints p κ :=
+  List.map (Expr.castLE h)
+
+@[simp] theorem maxDegree_castLE (c : Constraints p ι) (h : ι ≤ κ) :
+    maxDegree (c.castLE h) = maxDegree c := by
+  simp [maxDegree, castLE, Function.comp_def]
+
+@[simp] theorem maxDegree_add (cs : Constraints p ι) (c : Expr p ι) :
+    (cs.add c).maxDegree = Nat.max cs.maxDegree c.maxDegree := by
+  sorry
+
+end Constraints
+
+/-!
+### Assignments
+-/
+
+/--
+`Assignments` is a store for the fresh variables introduced in the degree lowering.
+Each element of the list represents a fresh variable, where the element of the list
+is the defining expression for the fresh variable.
+-/
+def Assignments (p ι : Nat) :=
+  List (Expr p ι)
+
+namespace Assignments
+
+def castLE (h : ι ≤ κ := by grind) : Assignments p ι → Assignments p κ :=
+  List.map (Expr.castLE h)
+
+/--
+Convert a set of fresh variable assignments into a set of constraints.
+
+NOTE: this assumes that `ι` is large enough to contain all new fresh variables.
+
+ACTUALLY: **the current code is broken**, as we've lost the starting point of the
+fresh variables. Oops. That is, when we run `lowerDegreeToTwo`, we start the
+computation with `ι` free variables, and the process will add some `κ` fresh
+variables and return an Assignment set in `ι+κ` variables. We assume that
+`κ` is equal to the length of the assignments, but that is not quite what we do
+here. Currently, we just assume that the first assignment in `v` is variable `0`,
+but actually, it should be variable `ι`!
+-/
+def toConstraints (v : Assignments p ι) : Constraints p ι :=
+  if h : ι = 0 then
+    [] -- This should never happen!
+  else
+    letI : NeZero ι := by constructor; exact h
+    v.mapIdx fun i expr =>
+      expr.sub (.var <| Fin.ofNat _ i)
+
+def maxDegree (v : Assignments p ι) : Nat :=
+  v.toConstraints.maxDegree
+  -- v.map Expr.maxDegree |>.max? |>.getD 0
+
+@[simp] theorem maxDegree_castLE (v : Assignments p ι) (h : ι ≤ κ) :
+    (v.castLE h).maxDegree = v.maxDegree := by
+  sorry
+
+end Assignments
+
+/-!
+### LowerDegreeToTwo
+-/
+
+def Expr.lowerDegreeToTwo (vars : Assignments p ι) :
+    Expr p ι →
+      (κ : Nat) × Assignments p (ι + κ) × Expr p (ι + κ)
+  | e@(.var _) | e@(.const _) => ⟨0, vars, e⟩
+  | .add e₁ e₂ =>
+      let ⟨κ₁, v₁, e₁⟩ := e₁.lowerDegreeToTwo vars
+      let ⟨κ₂, v₂, e₂⟩ := e₂.castLE.lowerDegreeToTwo v₁
+
+      ⟨κ₁ + κ₂, v₂.castLE, .add e₁.castLE e₂.castLE⟩
+  | .sub e₁ e₂ =>
+      let ⟨κ₁, v₁, e₁⟩ := e₁.lowerDegreeToTwo vars
+      let ⟨κ₂, v₂, e₂⟩ := e₂.castLE.lowerDegreeToTwo v₁
+
+      ⟨κ₁ + κ₂, v₂.castLE, .sub e₁.castLE e₂.castLE⟩
+  | .mul e₁ e₂ =>
+      let ⟨κ₁, v₁, e₁⟩ := e₁.lowerDegreeToTwo vars
+
+      let ⟨ω₁, w₁, e₁⟩ :
+          Σ (κ : Nat) (newVars : Assignments p (ι + κ)), Expr p (ι + κ) :=
+        if e₁.maxDegree ≥ 2 then
+          let w₁ : Assignments .. := v₁.append [e₁]
+          -- introduce fresh variable y = e₁
+          ⟨κ₁ + 1, w₁.castLE, Expr.var (Fin.last _)⟩
+          -- TODO: this could check whether e₂ already has a variable in Assigments
+        else
+          ⟨_, v₁, e₁⟩
+
+      let ⟨κ₂, v₂, e₂⟩ := e₂.castLE.lowerDegreeToTwo w₁
+
+      let ⟨ω₂, w₂, e₂⟩ :
+          Σ (κ : Nat) (newVars : Assignments p (ι + ω₁ + κ)), Expr p (ι + ω₁ + κ) :=
+        if e₁.maxDegree + e₂.maxDegree > 2 then
+          let w₂ : Assignments .. := v₂.append [e₂]
+          -- introduce fresh variable z = e₂
+          ⟨κ₂ + 1, w₂.castLE, Expr.var (Fin.last _)⟩
+          -- TODO: this could check whether e₂ already has a variable in Assigments
+        else
+          ⟨κ₂, v₂.castLE, e₂.castLE⟩
+
+      ⟨ω₁ + ω₂, w₂.castLE, .mul e₁.castLE e₂.castLE⟩
+  termination_by e => sizeOf e
+
+def Constraints.lowerDegreeToTwo (c : Constraints p ι) :
+      Σ (κ : Nat), Constraints p (ι + κ) :=
+  let ⟨κ, vars, c⟩ := go ⟨0, [], []⟩ c
+  let c := c ++ vars.toConstraints
+  ⟨κ, c⟩
+where
+  go : (κ : Nat) × Assignments p (ι + κ) × (Constraints p (ι + κ))
+      → Constraints p ι
+      → (κ : Nat) × Assignments p (ι + κ) × (Constraints p (ι + κ)) :=
+    List.foldl fun ⟨κ, vars, c⟩ expr =>
+      let ⟨κ', vars', expr'⟩ := expr.castLE.lowerDegreeToTwo vars
+      let c : Constraints p (ι + (κ + κ')) := c.castLE
+      ⟨κ + κ', vars'.castLE, c.add expr'.castLE⟩
 
 
-example (env : Environment p 3) :
-    LowerOrder.eval env → HigherOrder.eval env.restrict := by
-  unfold LowerOrder HigherOrder
-  simp only [Constraints.eval, Fin.isValue, List.all_cons, Expr.eval, Nat.cast_one, List.all_nil,
-    Bool.and_true, Bool.and_eq_true, beq_iff_eq, Environment.restrict, Fin.castLE_zero]
-  grind
+@[simp]
+theorem Constraints.lowerDegreeToTwo.go_nil
+    (κ : Nat) (as : Assignments p (ι + κ)) (csNew : Constraints p (ι + κ)):
+    Constraints.lowerDegreeToTwo.go ⟨κ, as, csNew⟩ [] = ⟨κ, as, csNew⟩ := rfl
+
+@[simp]
+theorem Constraints.lowerDegreeToTwo.go_cons
+    (κ : Nat) (as : Assignments p (ι + κ)) (csNew : Constraints p (ι + κ))
+    (c : Expr p ι) (cs : Constraints p ι) :
+    Constraints.lowerDegreeToTwo.go ⟨κ, as, csNew⟩ (c :: cs) =
+      let ⟨κ', as', expr'⟩ := (c.castLE.lowerDegreeToTwo as)
+      let res :=  Constraints.lowerDegreeToTwo.go ⟨κ + κ', as'.castLE, csNew.castLE.add expr'.castLE⟩ cs
+      res
+      := by rfl
+
+
+-- lemma:
+-- at any point in the fold, if the accumulator has all stuff of degree <= 2,
+-- and kappa is well formed (whatever that means), then the result of the
+-- fold will also have all stuff of degree <= 2.
+
+
+theorem isRefinedBy_lowerDegreeby
+    (c : Constraints p ι) {κ c'} (h : c.lowerDegreeToTwo = ⟨κ, c'⟩) :
+    c ⊑ c' := by
+  sorry
+
+
+theorem Constraints.lowerDegreeToTwo_cons (c : Expr p ι) (cs : Constraints p ι) :
+    Constraints.lowerDegreeToTwo.go ⟨k, vars, newCs⟩ (c :: cs) = ⟨k', vars', cs'⟩
+    ↔ ∃ d ds,
+        cs' = d :: ds := by
+  simp only [lowerDegreeToTwo.go_cons]
+  sorry
+
+theorem Expr.maxDegree_lowerDegree {e : Expr p ι}
+    (h_vars : vars.maxDegree ≤ 2) :
+    e.lowerDegreeToTwo vars = ⟨κ', vars', e'⟩
+    → vars'.maxDegree ≤ 2 ∧ e'.maxDegree ≤ 2 := by
+  intro h
+  fun_induction lowerDegreeToTwo vars e <;> simp only [Sigma.mk.injEq] at h
+  case case1 =>
+    rcases h with ⟨rfl, h⟩
+    simp only [Nat.add_zero, heq_eq_eq, Prod.mk.injEq] at h
+    rcases h with ⟨rfl, rfl⟩
+    simp [maxDegree, h_vars]
+  case case2 =>
+    rcases h with ⟨rfl, h⟩
+    simp only [Nat.add_zero, heq_eq_eq, Prod.mk.injEq] at h
+    rcases h with ⟨rfl, rfl⟩
+    simp [maxDegree, h_vars]
+  case case3 ih₁ ih₂ =>
+    rcases h with ⟨rfl, h⟩
+    simp only [heq_eq_eq, Prod.mk.injEq] at h
+    rcases h with ⟨rfl, rfl⟩
+    simp only [Assignments.maxDegree_castLE, maxDegree, maxDegree_castLE, sup_le_iff]
+    sorry
+  case case4 =>
+    rcases h with ⟨rfl, h⟩
+    simp only [heq_eq_eq, Prod.mk.injEq] at h
+    rcases h with ⟨rfl, rfl⟩
+    simp only [Assignments.maxDegree_castLE, maxDegree, maxDegree_castLE, sup_le_iff]
+
+    sorry
+  case case5 =>
+    sorry
+
+theorem Expr.maxDegree_lowerDegree₁ {e : Expr p ι}
+    (h_vars : vars.maxDegree ≤ 2) :
+    (e.lowerDegreeToTwo vars).2.1.maxDegree ≤ 2 := by
+  generalize hr : e.lowerDegreeToTwo vars = res
+  apply (maxDegree_lowerDegree h_vars hr).1
+
+theorem Expr.maxDegree_lowerDegree₂ (e : Expr p ι)
+    (h_vars : vars.maxDegree ≤ 2) :
+    (e.lowerDegreeToTwo vars).2.2.maxDegree ≤ 2 := by
+  generalize hr : e.lowerDegreeToTwo vars = res
+  apply (maxDegree_lowerDegree h_vars hr).2
+
+open Assignments in
+theorem Constraints.maxDegree_lowerDegree
+    (cs : Constraints p ι) (h : cs.lowerDegreeToTwo = ⟨κ, cs'⟩) :
+    cs'.maxDegree ≤ 2 := by
+  suffices ∀ {κ₀ vars₀ cs₀ κ' vars' cs'},
+    lowerDegreeToTwo.go ⟨κ₀, vars₀, cs₀⟩ cs = ⟨κ', vars', cs'⟩
+    → vars₀.maxDegree ≤ 2
+    → cs₀.maxDegree ≤ 2
+    → vars'.maxDegree ≤ 2 ∧ cs'.maxDegree ≤ 2
+  by
+    simp only [lowerDegreeToTwo] at h
+    generalize hr : (lowerDegreeToTwo.go ⟨0, ([], [])⟩ cs) = res at h
+    rcases h with ⟨rfl, rfl⟩
+    stop
+    apply this 0 [] [] κ _ cs' h
+  clear h
+  intro κ₀ vars₀ cs₀ κ' vars' cs' h_eq h_degree_vars₀ h_degree_cs₀
+  induction cs generalizing κ₀
+  case nil =>
+    simp only [lowerDegreeToTwo.go_nil, Sigma.mk.injEq] at h_eq
+    rcases h_eq with ⟨rfl, h_eq⟩
+    simp only [heq_eq_eq, Prod.mk.injEq] at h_eq
+    rcases h_eq with ⟨rfl, rfl⟩
+    and_intros <;> assumption
+  case cons c cs ih =>
+    simp only [lowerDegreeToTwo.go_cons] at h_eq
+    apply ih h_eq
+    · simpa using Expr.maxDegree_lowerDegree₁ (by assumption)
+    · simp only [maxDegree_add, maxDegree_castLE, Expr.maxDegree_castLE, sup_le_iff]
+      and_intros
+      · assumption
+      · apply Expr.maxDegree_lowerDegree₂
